scheduler/SchM.v
@@ -1,0 +1,81 @@
+(* Require Import CRIS.
+Require Import SchHeader.
+
+Definition thpool : Type := list (nat * option SAny.t).
+
+Module SchM. Section SchM.
+  Context `{!crisG Γ Σ α β τ _S _I, !concG}.
+
+  Definition scopes := [SCH].
+  Definition v_ths := SCH ↯ "ths".
+  Definition v_tid := SCH ↯ "tid".
+
+  Definition inner_spawn : string * SAny.t → itree crisE unit :=
+    λ '(fn, arg),
+      'rv : SAny.t <- ccallU fn arg;;
+      'ths : thpool <- cgetU v_ths;;
+      'tid : nat <- cgetU v_tid;;
+      match ths !! tid with
+      | Some (stid, None) =>
+          let ths2 := <[tid := (stid, Some rv)]> ths in
+          cput v_ths ths2;;;
+          Sch.terminate
+      | _ => triggerUB
+      end.
+
+  Definition spawn : string * SAny.t → itree crisE nat :=
+    λ '(fn, arg),
+      'ths : thpool <- cgetU v_ths;;
+      new_stid <- trigger (Spawn SchHdr._spawn (fn, arg)↑);;
+      let new_tid : nat := length ths in
+      cput v_ths (<[new_tid := (new_stid, None)]> ths);;;
+      Ret new_tid.
+
+  Definition yield : unit → itree crisE unit :=
+    λ _,
+      'ths : thpool <- cgetU v_ths;;
+      '(exist _ ntid _) :_ <- trigger (Choose {ntid : nat | ntid < length ths});;
+      (* Sanity check *)
+      tid <- trigger GetTid;;
+      'mtid : nat <- cgetU v_tid;;
+      match ths !! mtid with
+      | Some (stid, _) => if (decide (stid = tid)) then Ret () else triggerUB
+      | None => triggerUB
+      end;;;
+      trigger (Yield ntid);;;
+      cput v_tid mtid.
+
+  Definition join : nat → itree crisE (option SAny.t) :=
+    λ tid,
+      (* possibly infinite loop while waiting for the thread to terminate *)
+      orv <- (iterC (λ _,
+        'ths : thpool <- cgetU v_ths;;
+        match ths !! tid with
+        | None => Ret (inr None)
+        | Some (_, Some rv) => Ret (inr (Some rv))
+        | Some (_, None) => '() : _ <- ccallU SchHdr.yield tt;; Ret (inl tt)
+        end
+      ) tt);;
+      Ret orv.
+
+  Definition get_tid : unit → itree crisE nat :=
+    λ _, cgetN v_tid.
+
+  Definition fnsems : fnsems_type :=
+    [(Some SchHdr._spawn,  (false, wmask_all, scopes, (None, cfunU inner_spawn)));
+     (Some SchHdr.spawn,   (false, wmask_all, scopes, (None, cfunU spawn)));
+     (Some SchHdr.yield,   (false, wmask_all, scopes, (None, cfunU yield)));
+     (Some SchHdr.join,    (false, wmask_all, scopes, (None, cfunU join)));
+     (Some SchHdr.get_tid, (false, wmask_all, scopes, (None, cfunU get_tid)))].
+
+  Program Definition smod: SMod.t :=
+  {|
+    SMod.scopes := scopes;
+    SMod.fnsems := fnsems;
+    SMod.initial_st := [(v_ths, ([(0, None)] : thpool)↑); (v_tid, 0↑)];
+  |}.
+  Solve All Obligations with prove_scope.
+  Next Obligation. prove_nodup. Qed.
+
+  Definition t := Seal.sealing CRIS (SMod.to_mod sp_none smod).
+End SchM. End SchM. *)
