theories/common/ConcRA.v
@@ -52,5 +52,5 @@ Section preds.
   Qed.
 End preds.
 
-Notation "'TID' tid" := (TidToken tid) (at level 20, tid at level 1, format "TID tid").
-Notation "'YIELD' tid" := (YieldToken tid) (at level 20, tid at level 1, format "YIELD tid").
+Notation "'TID' tid" := (TidToken tid) (at level 20, tid at level 1, format "TID  tid").
+Notation "'YIELD' tid" := (YieldToken tid) (at level 20, tid at level 1, format "YIELD  tid").
